propagate step 2.2 finish

src/Std/Tactic/BVDecide/Bitblast/BVExpr/Circuit/Impl.lean
@@ -10,16 +10,3 @@ import Std.Tactic.BVDecide.Bitblast.BVExpr.Circuit.Impl.Substructure
 This module contains the implementation of a bitblaster for general `BitVec` problems with boolean
 substructure (`BVLogicalExpr`). It is the main entrypoint into the bitblasting framework.
 -/
-
-namespace Std.Tactic.BVDecide
-
-open Std.Sat
-
-namespace BVLogicalExpr
-
-def bitblast (expr : BVLogicalExpr) : AIG.Entrypoint BVBit :=
-  ofBoolExprCached expr
-
-end BVLogicalExpr
-
-end Std.Tactic.BVDecide
